Change future idiom to handle multiple outbound promises (#539)
Added a new channel idiom for multiple independent promises where a
single consumer collects all results without caring about completion
order.

The key challenge is that completion order is non-deterministic. This
forces extensive permutation reasoning throughout proofs to track which
contracts remain pending and prove the final result contains exactly the
expected values.

I proved the Google search example from
https://go.dev/talks/2012/concurrency.slide#46 demonstrating the pattern
with three concurrent workers and permutation-based correctness. Proving
this idiom seems unavoidably painful but perhaps we can add some helpers
if this comes up a lot in the future.

Also updated the higher-order example to use mfuture and removed the
single-future idiom since both handoff and this idiom can replace it.

Regoose for https://github.com/goose-lang/goose/pull/172

new/proof/github_com/goose_lang/goose/testdata/examples/channel.v
@@ -1,10 +1,11 @@
 From New.proof Require Export proof_prelude.
 From New.proof.github_com.goose_lang.goose.model.channel
-     Require Import idiom.base handoff future spsc done dsp dsp_proofmode mpmc join handshake.
+Require Import idiom.base handoff future spsc done dsp dsp_proofmode mpmc join handshake.
 From New.proof Require Import strings time sync.
 From New.generatedproof.github_com.goose_lang.goose.testdata.examples Require Import channel.
 From iris.base_logic Require Import ghost_map.
 From New.golang Require Import theory.
+From New.proof Require Import strings.
 From iris.algebra Require Import gmultiset.
 
 Import New.code.github_com.goose_lang.goose.testdata.examples.channel.chan_spec_raw_examples.
@@ -825,40 +826,55 @@ End select_panic.
 
 Section higher_order_example.
 
-Definition do_request (r: chan_spec_raw_examples.request.t) γfut (Q: go_string → iProp Σ) : iProp Σ :=
-  "Hf" ∷ WP #r.(chan_spec_raw_examples.request.f') #() {{ λ v, ∃ (s: go_string), ⌜v = #s⌝ ∗ Q s }} ∗
-  "#Hfut" ∷ is_future γfut r.(chan_spec_raw_examples.request.result') Q ∗
-  "Hfut_tok" ∷ fulfill_token γfut.
+Context `{!ghost_map.ghost_mapG Σ gname (go_string → iProp Σ)}.
+Context `{!inG Σ unitR}.
 
-Definition await_request r γfut (Q: go_string → iProp Σ) : iProp Σ :=
-  "#Hfut" ∷ is_future γfut r.(chan_spec_raw_examples.request.result') Q ∗
-  "Hfut_await" ∷ await_token γfut.
+Definition do_request (r: request.t) γfut (Q: go_string → iProp Σ) : iProp Σ :=
+  "Hf" ∷ WP #r.(request.f') #() {{ λ v, ∃ (s: go_string), ⌜v = #s⌝ ∗ Q s }} ∗
+  "#Hfut" ∷ is_future (V:=go_string)  γfut r.(request.result') ∗
+  "Hpromise" ∷ Fulfill (V:=go_string)  γfut Q.
+
+Definition await_request (r: request.t) γfut (Q: go_string → iProp Σ) : iProp Σ :=
+  "#Hfut" ∷ is_future (V:=go_string) γfut r.(request.result') ∗
+  "HAwait" ∷ Await (V:=go_string) γfut [Q].
 
 Lemma wp_mkRequest {f: func.t} (Q: go_string → iProp Σ) :
   {{{ is_pkg_init chan_spec_raw_examples ∗ WP #f #() {{ λ v, ∃ (s: go_string), ⌜v = #s⌝ ∗ Q s }} }}}
     @! chan_spec_raw_examples.mkRequest #f
-  {{{ γfut r, RET #r; do_request r γfut Q ∗ await_request r γfut Q }}}.
-Proof.
+  {{{ γfut (r: request.t), RET #r; do_request r γfut Q ∗ await_request r γfut Q }}}.
+  Proof using H ext ffi ffi_interp0 ffi_semantics0 hG inG0 package_sem sem Σ.
   wp_start as "Hf".
   wp_auto.
   wp_apply chan.wp_make2; first done.
   iIntros (ch γ) "(His & _Hcap & Hown)".
-  simpl. (* for decide *)
-  iMod (start_future with "His Hown") as (γfuture) "(#Hfut & Hawait & Hfulfill)".
+  simpl.
+  iMod (start_future (V:=go_string)  (t:=go.string) (ghost_mapG0:=H)   ch γ (chanstate.Buffered []) with "[$His] [$Hown]") as (γfuture) "(#Hfut & HAwait)".
+  { right. done. }
+  iMod (future_alloc_promise (V:=go_string) (t:=go.string) γfuture ch Q [] with "Hfut HAwait") as "(Hpromise & HAwait)".
   wp_auto.
   iApply "HΦ".
-  iFrame "Hfut ∗".
+  iFrame "Hfut Hf Hpromise HAwait".
 Qed.
 
 #[local] Lemma wp_get_response r γfut Q :
   {{{ await_request r γfut Q }}}
     chan.receive go.string #r.(chan_spec_raw_examples.request.result')
   {{{ (s: go_string), RET (#s, #true); Q s }}}.
-Proof.
+  Proof using H ext ffi ffi_interp0 ffi_semantics0 hG inG0 package_sem sem Σ.
+
   wp_start as "Hawait". iNamed "Hawait".
-  wp_apply (wp_future_await with "[$Hfut $Hfut_await]").
-  iIntros (v) "HQ".
-  iApply "HΦ". done.
+  wp_apply (wp_future_await with "[$Hfut $HAwait]").
+  iIntros (v P pre post) "(%Hsplit & HP & _HAwait)".
+  destruct pre as [|? pre']; simpl in Hsplit.
+  - injection Hsplit as <-. 
+    destruct post as [|? post']; last done.
+    iApply "HΦ". iFrame.
+  -  iApply "HΦ". exfalso.
+    assert (length [Q] = length (u :: pre' ++ P :: post)) as Hlen by (rewrite Hsplit; done).
+    simpl in Hlen.
+    rewrite app_length in Hlen.
+    simpl in Hlen.
+    lia.
 Qed.
 
 Definition is_request_chan γ (ch: loc): iProp Σ :=
@@ -868,7 +884,7 @@ Lemma wp_ho_worker γ ch :
   {{{ is_pkg_init chan_spec_raw_examples ∗ is_request_chan γ ch }}}
     @! chan_spec_raw_examples.ho_worker #ch
   {{{ RET #(); True }}}.
-Proof.
+  Proof using H ext ffi ffi_interp0 ffi_semantics0 hG inG0 package_sem sem Σ.
   wp_start as "#His".
   rewrite /is_request_chan.
   wp_auto.
@@ -884,7 +900,7 @@ Proof.
   iIntros (v) "HQ".
   iDestruct "HQ" as (s) "[-> HQ]".
   wp_auto.
-  wp_apply (wp_future_fulfill with "[$Hfut $Hfut_tok HQ]").
+  wp_apply (wp_future_fulfill with "[$Hfut $Hpromise HQ]").
   { done. }
   wp_for_post.
   iFrame.
@@ -894,7 +910,7 @@ Lemma wp_HigherOrderExample :
   {{{ is_pkg_init chan_spec_raw_examples }}}
     @! chan_spec_raw_examples.HigherOrderExample #()
   {{{ (s:slice.t), RET #s; s ↦* ["hello world"%go; "HELLO"%go; "world"%go] }}}.
-Proof.
+  Proof using H ext ffi ffi_interp0 ffi_semantics0 hG inG0 package_sem sem Σ.
   wp_start.
   wp_auto.
   wp_apply chan.wp_make1.
@@ -1503,4 +1519,581 @@ Qed.
 
 End broadcast_example_proof.
 
+Section google_example.
+
+Context `{!chan_idiomG Σ go_string}.
+Context `{!ghost_map.ghost_mapG Σ gname (go_string → iProp Σ)}.
+  #[local] Existing Instance H.
+Context `{!inG Σ unitR}.
+
+Lemma wp_Web (q : go_string) :
+  {{{ is_pkg_init chan_spec_raw_examples }}}
+    @! chan_spec_raw_examples.Web #q
+  {{{ RET #(q ++ ".html"%go); True }}}.
+Proof. wp_start. wp_auto. iApply "HΦ". done. Qed.
+
+Lemma wp_Image (q : go_string) :
+  {{{ is_pkg_init chan_spec_raw_examples }}}
+    @! chan_spec_raw_examples.Image #q
+  {{{ RET #(q ++ ".png"%go); True }}}.
+Proof. wp_start. wp_auto. iApply "HΦ". done. Qed.
+
+Lemma wp_Video (q : go_string) :
+  {{{ is_pkg_init chan_spec_raw_examples }}}
+    @! chan_spec_raw_examples.Video #q
+  {{{ RET #(q ++ ".mp4"%go); True }}}.
+Proof. wp_start. wp_auto. iApply "HΦ". done. Qed.
+
+
+Definition google_expected (q: go_string) : list go_string :=
+  [ q ++ ".html"%go; q ++ ".png"%go; q ++ ".mp4"%go ].
+
+
+Inductive kind := KWeb | KImg | KVid.
+
+Definition kind_eq_dec : ∀ x y : kind, {x = y} + {x ≠ y}.
+Proof. decide equality. Defined.
+
+Definition value_of (q:go_string) (k:kind) : go_string :=
+  match k with
+  | KWeb => q ++ ".html"%go
+  | KImg => q ++ ".png"%go
+  | KVid => q ++ ".mp4"%go
+  end.
+
+Definition pure_contract_of (q:go_string) (k:kind) : go_string → Prop :=
+  λ v, v = value_of q k.
+
+Definition contract_of (q:go_string) (k:kind) : go_string → iProp Σ :=
+  λ v, ⌜pure_contract_of q k v⌝%I.
+
+Lemma pure_contract_of_inj (q:go_string) (k1 k2:kind) :
+  pure_contract_of q k1 = pure_contract_of q k2 → k1 = k2.
+Proof.
+  
+  intro Heq.
+  destruct k1, k2; try done.
+  all: exfalso.
+  all: 
+    set v := value_of q KWeb.
+    {
+    have Heqv : pure_contract_of q KWeb v = pure_contract_of q KImg v by (exact (f_equal (fun f => f v) Heq)).
+    rewrite /pure_contract_of in Heqv.
+     subst v.
+  unfold value_of in Heqv.
+
+  symmetry in Heqv.
+  assert (q ++ ".html"%go ≠ q ++ ".png"%go).
+  {
+   destruct q.
+   {
+    set_solver.
+   }
+   set_solver. 
+  }
+  {
+    assert ((q ++ ".html"%go = q ++ ".html"%go)).
+    {
+      done.
+    }
+  assert (q ++ ".html"%go = q ++ ".png"%go).
+  { rewrite Heqv. reflexivity. }
+  congruence.
+  }
+    }
+      {
+    have Heqv : pure_contract_of q KWeb v = pure_contract_of q KVid v by (exact (f_equal (fun f => f v) Heq)).
+    rewrite /pure_contract_of in Heqv.
+     subst v.
+  unfold value_of in Heqv.
+
+  symmetry in Heqv.
+  assert (q ++ ".html"%go ≠ q ++ ".mp4"%go).
+  {
+   destruct q.
+   {
+    set_solver.
+   }
+   set_solver. 
+  }
+  {
+    assert ((q ++ ".html"%go = q ++ ".html"%go)).
+    {
+      done.
+    }
+  assert (q ++ ".html"%go = q ++ ".mp4"%go).
+  { rewrite Heqv. reflexivity. }
+  congruence.
+  }
+    }
+    {
+    have Heqv : pure_contract_of q KImg v = pure_contract_of q KWeb v by (exact (f_equal (fun f => f v) Heq)).
+    rewrite /pure_contract_of in Heqv.
+     subst v.
+  unfold value_of in Heqv.
+
+  symmetry in Heqv.
+  assert (q ++ ".html"%go ≠ q ++ ".png"%go).
+  {
+   destruct q.
+   {
+    set_solver.
+   }
+   set_solver. 
+  }
+  {
+    assert ((q ++ ".html"%go = q ++ ".html"%go)).
+    {
+      done.
+    }
+  assert (q ++ ".html"%go = q ++ ".png"%go).
+  { 
+    rewrite Heqv in H1.
+  done.
+  }
+  congruence.
+  }
+
+    }
+
+       {
+  unfold pure_contract_of in Heq.
+  assert (value_of q KImg = value_of q KVid) as Hbad.
+  { apply (f_equal (fun f => f (value_of q KImg))) in Heq.
+    unfold value_of in Heq. simpl in Heq.
+    symmetry in Heq.
+    assert (q ++ ".png"%go = q ++ ".mp4"%go).
+    { rewrite Heq. reflexivity. }
+    assumption.
+  }
+  
+  unfold value_of in Hbad. simpl in Hbad.
+  
+  assert (q ++ ".png"%go ≠ q ++ ".mp4"%go).
+  { intros Heq_bad.
+    set_solver.
+  }
+  congruence.
+       }
+         {
+  unfold pure_contract_of in Heq.
+  
+  assert (value_of q KVid = value_of q KWeb) as Hbad.
+  { apply (f_equal (fun f => f (value_of q KVid))) in Heq.
+    unfold value_of in Heq. simpl in Heq.
+    symmetry in Heq.
+    assert (q ++ ".mp4"%go = q ++ ".html"%go).
+    { rewrite Heq. reflexivity. }
+    assumption.
+  }
+  
+  unfold value_of in Hbad. simpl in Hbad.
+  assert (q ++ ".mp4"%go ≠ q ++ ".html"%go).
+  { intros Heq_bad.
+    set_solver.
+  }
+  congruence.
+       }
+        {
+  unfold pure_contract_of in Heq.
+  
+  assert (value_of q KVid = value_of q KImg) as Hbad.
+  { apply (f_equal (fun f => f (value_of q KVid))) in Heq.
+    unfold value_of in Heq. simpl in Heq.
+    symmetry in Heq.
+    assert (q ++ ".mp4"%go = q ++ ".png"%go).
+    { rewrite Heq. reflexivity. }
+    assumption.
+  }
+  
+  unfold value_of in Hbad. simpl in Hbad.
+  assert (q ++ ".mp4"%go ≠ q ++ ".png"%go).
+  { intros Heq_bad.
+    set_solver.
+  }
+  congruence.
+       }
+Qed.
+
+Definition pendingk : list kind := [KWeb; KImg; KVid].
+
+Lemma pendingk_nodup : NoDup pendingk.
+Proof. unfold pendingk. repeat constructor; set_solver. Qed.
+
+Lemma contract_of_sound (q:go_string) (k:kind) (v:go_string) :
+  contract_of q k v ⊢ ⌜v = value_of q k⌝.
+Proof. iIntros "%Hv". iPureIntro. exact Hv. Qed.
+
+Lemma mem_map_contract_of (q:go_string) (remk:list kind) (P:go_string→iProp Σ) :
+  P ∈ map (contract_of q) remk →
+  ∃ k, k ∈ remk ∧ P = contract_of q k.
+Proof.
+  intro HP.
+  rewrite -(list_fmap_map (contract_of q) remk) in HP.
+  apply (proj1 (list_elem_of_fmap _ _ _)) in HP.
+  destruct HP as (k & -> & Hk). eauto.
+Qed.
+
+Lemma delete_middle {A} (l1 : list A) (x : A) (l2 : list A) :
+  delete (length l1) (l1 ++ x :: l2) = l1 ++ l2.
+Proof.
+  induction l1 as [|a l1 IH]; simpl; [done|].
+  by rewrite IH.
+Qed.
+
+Lemma wp_Google (q : go_string) :
+  {{{ is_pkg_init chan_spec_raw_examples }}}
+    @! chan_spec_raw_examples.Google #q
+  {{{ (sl : slice.t), RET #sl;
+      ∃ xs, sl ↦* xs ∗ ⌜xs ≡ₚ google_expected q⌝ }}}.
+Proof using All.
+  wp_start.
+  wp_auto.
+
+  wp_apply (chan.wp_make2 (W64 3)); first done.
+  iIntros (c γch) "(#Hchan & %Hcap3 & Hown)".
+  simpl in *.
+
+  iMod (start_future
+          (V:=go_string)
+          (t:=go.string)
+          (ghost_mapG0:=H)
+          c γch (chanstate.Buffered [])
+        with "[$Hchan] [$Hown]") as (γmf) "(#Hmf & HAwait)".
+  { right. done. }
+
+  wp_auto.
+
+  iMod (future_alloc_promise γmf c (contract_of q KWeb) []
+        with "[$Hmf] [$HAwait]") as "(Hprom_web & HAwait)".
+  iMod (future_alloc_promise γmf c (contract_of q KImg) _
+        with "[$Hmf] [$HAwait]") as "(Hprom_img & HAwait)".
+  iMod (future_alloc_promise γmf c (contract_of q KVid) _
+        with "[$Hmf] [$HAwait]") as "(Hprom_vid & HAwait)".
+
+  simpl.
+  iPersist "c query".
+
+  wp_apply (wp_fork with "[Hprom_web]").
+  {
+    wp_auto.
+    wp_apply (wp_Web q).
+    wp_apply (wp_future_fulfill
+                (V:=go_string)
+                (t:=go.string)
+                (ghost_mapG0:=H)
+                γmf c (value_of q KWeb)
+              with "[$Hmf $Hprom_web]").
+    { iPureIntro. reflexivity. }
+    done.
+  }
+
+  wp_apply (wp_fork with "[Hprom_img]").
+  {
+    wp_auto.
+    wp_apply (wp_Image q).
+    wp_apply (wp_future_fulfill
+                (V:=go_string)
+                (t:=go.string)
+                (ghost_mapG0:=H)
+                γmf c (value_of q KImg)
+              with "[$Hmf $Hprom_img]").
+    { iPureIntro. reflexivity. }
+    done.
+  }
+
+  wp_apply (wp_fork with "[Hprom_vid]").
+  {
+    wp_auto.
+    wp_apply (wp_Video q).
+    wp_apply (wp_future_fulfill
+                (V:=go_string)
+                (t:=go.string)
+                (ghost_mapG0:=H)
+                γmf c (value_of q KVid)
+              with "[$Hmf $Hprom_vid]").
+    { iPureIntro. reflexivity. }
+    done.
+  }
+
+  wp_apply (wp_slice_make3 (V:=go_string) (t:=go.string)).
+  { word. }
+
+  iIntros (sl) "[Hsl [Hcap_sl %Hcap]]".
+  wp_auto.
+
+  iAssert (∃ (i : nat) (xs : list go_string)
+                  (donek remk : list kind) (sl0 : slice.t),
+      "i"            ∷ i_ptr ↦ W64 i ∗
+      "results"      ∷ results_ptr ↦ sl0 ∗
+      "Hsl"          ∷ sl0 ↦* xs ∗
+      "Hcap"         ∷ own_slice_cap go_string sl0 (DfracOwn 1) ∗
+      "HAwait"       ∷ Await (V:=go_string) γmf (map (contract_of q) remk) ∗
+      "%Hlen"        ∷ ⌜length xs = i⌝ ∗
+      "%Hi"          ∷ ⌜i ≤ 3⌝ ∗
+      "%Hrem"        ∷ ⌜length remk = 3 - i⌝ ∗
+      "%Hnodup_rem"  ∷ ⌜NoDup remk⌝ ∗
+      "%Hsplit"      ∷ ⌜pendingk ≡ₚ donek ++ remk⌝ ∗
+      "%Hperm"       ∷ ⌜xs ≡ₚ map (value_of q) donek⌝
+    )%I
+    with "[i results Hsl Hcap_sl HAwait]" as "IH".
+  {
+    iFrame.
+    iExists 0.
+    iExists ([] : list kind).
+    iFrame.
+    iExists ([KWeb; KImg; KVid]).
+    iSplitL "HAwait".
+    { iNamedAccu. }
+    iFrame.
+    repeat (iSplit; [iPureIntro; try reflexivity; try lia;
+                     auto using pendingk_nodup|]).
+    iPureIntro. simpl. reflexivity.
+  }
+
+  wp_for "IH".
+  wp_if_destruct.
+
+  - wp_apply (wp_future_await
+                (V:=go_string)
+                (t:=go.string)
+                (ghost_mapG0:=H)
+                γmf c (map (contract_of q) remk)
+              with "[$Hmf HAwait]").
+    { iNamedAccu. }
+
+    iIntros (v P pre post) "(%HsplitP & HPv & HAwait')".
+
+    have HPmem : P ∈ map (contract_of q) remk
+      by (rewrite HsplitP; set_solver).
+    destruct (mem_map_contract_of q remk P HPmem)
+      as (k & Hkin & ->).
+    iDestruct (contract_of_sound q k v with "HPv") as %->.
+
+    wp_auto.
+
+    wp_apply wp_slice_literal as "% Hsl1".
+    { iIntros. wp_auto. iFrame. }
+
+    wp_apply (wp_slice_append with "[$Hsl $Hcap $Hsl1]").
+    iIntros (sl') "[Hsl' Hcap']".
+    wp_auto.
+
+    set j := length pre.
+    set remk' := delete j remk.
+
+    have Hj_lt_map : j < length (map (contract_of q) remk).
+    {
+      subst j.
+      rewrite HsplitP.
+      rewrite app_length /=.
+      lia.
+    }
+
+    have Hj_lt : j < length remk.
+    {
+      rewrite length_map in Hj_lt_map.
+      done.
+    }
+
+    have Hlook_map :
+      (map (contract_of q) remk) !! j = Some (contract_of q k).
+    {
+      subst j.
+      rewrite HsplitP.
+      rewrite lookup_app_r; last lia.
+      replace (length pre - length pre) with 0 by lia.
+      simpl. done.
+    }
+
+    apply (list_lookup_fmap_Some
+             (contract_of q) remk j (contract_of q k))
+      in Hlook_map as (k0 & Hk0 & Hk0eq).
+
+    apply (f_equal (fun f => f (value_of q k0))) in Hk0.
+    simpl in Hk0.
+
+    iAssert (⌜value_of q k0 = value_of q k⌝)%I as "%Hbad".
+    {
+      unfold contract_of, pure_contract_of in Hk0.
+      iEval (rewrite Hk0). done.
+    }
+
+    have Heq_k0_k : k0 = k.
+    {
+      apply (pure_contract_of_inj q).
+      unfold contract_of, pure_contract_of in Hk0.
+      unfold contract_of, pure_contract_of.
+      rewrite Hbad.
+      done.
+    }
+
+    have Hlook_remk : remk !! j = Some k
+      by (replace k with k0 by done; done).
+
+    have Hdecomp :
+      take j remk ++ k :: drop (S j) remk = remk
+      by exact (take_drop_middle remk j k Hlook_remk).
+
+    have Hrem' : length remk' = 3 - S (length xs).
+    {
+      rewrite /remk' length_delete;
+        [|by apply lookup_lt_is_Some_2].
+      lia.
+    }
+
+    have Hmap_remk' :
+      map (contract_of q) remk' = pre ++ post.
+    {
+      subst remk' j.
+      rewrite -!list_fmap_map list_fmap_delete list_fmap_map.
+      rewrite HsplitP delete_middle.
+      done.
+    }
+
+    set donek' := donek ++ [k].
+
+    have Hsplit' :
+      pendingk ≡ₚ donek' ++ remk'.
+    {
+      unfold donek', remk'.
+      subst j.
+      eapply Permutation_trans; [exact Hsplit|].
+      rewrite (delete_take_drop remk) -Hdecomp.
+      repeat rewrite -app_assoc.
+      simpl.
+      apply Permutation_app_head.
+      rewrite Permutation_middle Hdecomp.
+      rewrite Hdecomp.
+      done.
+    }
+
+    have Hperm' :
+      (xs ++ [value_of q k]) ≡ₚ map (value_of q) donek'.
+    {
+      unfold donek'.
+      rewrite map_app /=.
+      etransitivity; [|reflexivity].
+      rewrite Hperm.
+      reflexivity.
+    }
+
+    have Hnodup_rem' : NoDup remk'.
+    {
+      apply (sublist_NoDup _ _ Hnodup_rem).
+      apply sublist_delete.
+    }
+
+    wp_for_post.
+    iFrame "HΦ".
+    iExists (S (length xs)),
+            (xs ++ [value_of q k]),
+            donek', remk', sl'.
+    iFrame "#%".
+    iFrame.
+
+    iSplitL "i".
+    {
+      replace (W64 (S (length xs)))
+        with (w64_word_instance.(word.add)
+                (W64 (length xs)) (W64 1))
+        by word.
+      done.
+    }
+
+    iDestruct "Hcap'" as "[Hcap Hsl]".
+    iFrame.
+
+    iSplitL "HAwait'".
+    { rewrite Hmap_remk'. done. }
+
+    repeat (iSplit;
+            [iPureIntro;
+             auto;
+             try (rewrite length_app singleton_length; lia)|]).
+    iPureIntro. lia.
+
+  - iApply "HΦ".
+    iExists xs.
+    iFrame "Hsl".
+    iPureIntro.
+
+    have Hlenxs : length xs = 3.
+    {
+      have : ¬ length xs < 3 by (intro; apply n; word).
+      lia.
+    }
+
+    have Hremk_nil : remk = [].
+    {
+      apply length_zero_iff_nil.
+      rewrite Hrem.
+      assert (length xs = 3) by exact Hlenxs.
+      lia.
+    }
+
+    have Hdone : pendingk ≡ₚ donek.
+    {
+      subst remk.
+      rewrite app_nil_r in Hsplit.
+      done.
+    }
+
+    have Hmap :
+      map (value_of q) pendingk ≡ₚ
+      map (value_of q) donek :=
+      Permutation_map (value_of q) Hdone.
+
+    have Hexp :
+      map (value_of q) pendingk = google_expected q.
+    { reflexivity. }
+
+    etransitivity; [exact Hperm|].
+    eapply Permutation_trans.
+    { exact (Permutation_sym Hmap). }
+    rewrite Hexp.
+    apply Permutation_refl.
+
+    Unshelve.
+    all: try (typeclasses eauto).
+    all: try apply _; try apply sem; try apply go.string.
+
+    { simpl.
+      pose proof (_ : go.PredeclaredSemantics) as Hpre.
+      have Hunder :
+        sem.(go.sem_fn).(underlying) go.string = go.string :=
+        go.predeclared_underlying
+          (H:=sem.(go.sem_fn))
+          go.string
+          go.is_predeclared_string.
+      rewrite Hunder.
+      typeclasses eauto.
+    }
+
+    { simpl.
+      pose proof (_ : go.PredeclaredSemantics) as Hpre.
+      have Hunder :
+        sem.(go.sem_fn).(underlying) go.string = go.string :=
+        go.predeclared_underlying
+          (H:=sem.(go.sem_fn))
+          go.string
+          go.is_predeclared_string.
+      rewrite Hunder.
+      typeclasses eauto.
+    }
+
+    { simpl.
+      pose proof (_ : go.PredeclaredSemantics) as Hpre.
+      have Hunder :
+        sem.(go.sem_fn).(underlying) go.string = go.string :=
+        go.predeclared_underlying
+          (H:=sem.(go.sem_fn))
+          go.string
+          go.is_predeclared_string.
+      rewrite Hunder.
+      typeclasses eauto.
+    }
+Qed.
+
+End google_example.
 End proof.
